deps/poulet4/lib/P4automata/P4automaton.v
@@ -539,3 +539,74 @@ Proof.
     + apply close_interpolate_sound.
     + now apply bisimilar_with_leaps_implies_bisimilar_upto.
 Qed.
+
+Lemma follow_buffer
+  {a: p4automaton}
+  (s: states a)
+  (st: store a)
+  (buf buf': list bool)
+:
+  Datatypes.length buf + Datatypes.length buf' + 1 < size a s ->
+  follow (inl s, st, buf) buf' =
+  (inl s, st, buf ++ buf')
+.
+Proof.
+  induction buf' using rev_ind; intros.
+  - now rewrite follow_nil, app_nil_r.
+  - unfold follow.
+    rewrite fold_left_app.
+    fold (follow (inl s, st, buf) buf').
+    simpl fold_left.
+    rewrite IHbuf'.
+    + rewrite step_with_space.
+      * now rewrite app_assoc.
+      * rewrite app_length in *.
+        simpl in *.
+        lia.
+    + rewrite app_length in *.
+      simpl Datatypes.length in *.
+      lia.
+Qed.
+
+Lemma follow_exact
+  {a: p4automaton}
+  (s: states a)
+  (st: store a)
+  (buf buf': list bool)
+:
+  Datatypes.length buf' > 0 ->
+  Datatypes.length buf + Datatypes.length buf' = size a s ->
+  follow (inl s, st, buf) buf' =
+    let st' := update a s (buf ++ buf') st in
+    (transitions a s st', st', nil)
+.
+Proof.
+  intros.
+  destruct buf'.
+  - simpl Datatypes.length in H.
+    lia.
+  - revert s st buf b H H0.
+    induction buf'; intros.
+    + rewrite follow_cons, follow_nil.
+      unfold step.
+      rewrite app_length.
+      simpl Datatypes.length in *.
+      destruct (equiv_dec _ _); trivial.
+      exfalso; eapply c; auto.
+      
+    + rewrite follow_cons.
+      rewrite step_with_space.
+      rewrite IHbuf'.
+      * repeat f_equal;
+        rewrite <- app_assoc;
+        rewrite <- app_comm_cons;
+        rewrite app_nil_l;
+        easy.
+      * simpl Datatypes.length in *.
+        lia.
+      * rewrite app_length in *.
+        simpl Datatypes.length in *.
+        lia.
+      * simpl Datatypes.length in *.
+        lia.
+Qed.
